theorems/main.md
@@ -1,0 +1,60 @@
+```v
+Theorem absurd_well_founded_minimal {T} (P: T -> T -> Prop) (least other: T):
+  well_founded P
+  -> P least other
+  -> ~(P other least).
+Proof.
+intros.
+
+
+Qed.
+
+Section well_founded_compatibility.
+  Variable A B: Type.
+  Variable RA: A -> A -> Prop.
+  Variable RB: B -> B -> Prop.
+
+  Variable RB_well_founded: well_founded RB.
+  Variable f: A -> B.
+  Hypothesis H_compat_A: forall a1 a2: A, (RA a1 a2) -> (RB (f a1) (f a2)).
+  Hypothesis H_compat_B: forall a1 a2: A, (RB (f a1) (f a2)) -> (RA a1 a2).
+
+  Theorem yo:
+    forall min other, RB (f min) (f other) -> Acc RA min.
+  Proof.
+intros ?? HRB.
+apply H_compat_B in HRB.
+Hint Constructors Acc: core.
+
+
+  Qed.
+
+
+  Theorem well_founded_compat: well_founded RA.
+  Proof.
+constructor.
+
+unfold well_founded in *.
+constructor.
+intros.
+rename y into a1; rename a into a2.
+
+specialize (H_compat a1 a2).
+remember (f a1) as b1; remember (f a2) as b2.
+destruct H_compat as [H_compat_A H_compat_B].
+specialize (H_compat_A H) as ?.
+
+
+specialize (RB_well_founded b1) as Hb1.
+specialize (RB_well_founded b2) as Hb2.
+inversion Hb1.
+
+
+specialize (Acc_inv RB_well_founded).
+
+  Qed.
+
+Check RB_well_founded.
+
+EndSection well_founded_compatibility.
+```
